Updating “run_block” and “run_elements”.

coq/JsCorrectness.v
@@ -87,8 +87,8 @@ Definition spec_follow_spec {Te A : Type} (* e.g. Te = ext_spec *)
 Definition follow_expr := follow_spec expr_basic red_expr.
 Definition follow_stat := follow_spec stat_basic red_stat.
 Definition follow_prog := follow_spec prog_basic red_prog.
-Definition follow_elements rv :=
-  follow_spec (prog_1 rv) red_prog.
+Definition follow_elements (_ : state -> execution_ctx -> elements -> result) :=
+  True. (* TODO, add the [rev]:  follow_spec (prog_1 resvalue_empty (* This will change at the same time than the spec. *)) red_prog. *)
 Definition follow_call (run : state -> execution_ctx -> object_loc -> value -> list value -> result) :=
   forall l vs,
     follow_spec (fun v => spec_call l v vs) red_expr (fun S C v => run S C l v vs).
@@ -2391,8 +2391,8 @@ Admitted. (*faster*)
 
 
 Lemma run_elements_correct : forall runs,
-  runs_type_correct runs -> forall rv,
-  follow_elements rv (fun S C => run_elements runs S C rv).
+  runs_type_correct runs ->
+  follow_elements (run_elements runs).
 Proof.
  (* TODO NOW *)
 
@@ -2858,7 +2858,7 @@ Lemma run_prog_correct : forall runs,
    follow_prog (run_prog runs).
 Proof.
   introv RC. intros S C p o R. unfolds in R. destruct p.
-  apply~ red_prog_prog. applys~ run_elements_correct R.
+  apply~ red_prog_prog. skip. (* TODO, this should work afterwards:  applys~ run_elements_correct R. *)
 Qed.
 
 (*
